subset notation

model/Enum.v
@@ -5,6 +5,20 @@ Require Import Coq.Lists.ListSet.
 Require Import Coq.Lists.List.
 Require Import Psatz.
 
+(* TeX input mode notes:
+Sets
+∅ \emptyset
+∈ \in
+∪ \cup  
+⊂ \subset
+≃ \simeq
+
+Traces
+ε \epsilon
+⊕ \oplus
+⊏ \sqsubset
+≡ \equiv
+*)
 Ltac nliamega := try omega; try lia; try nia; fail "omega, lia and nia all failed".
 
 Inductive Value : Set :=
@@ -345,13 +359,14 @@ Section Sets.
         set_In x s2 /\ subset more s2
     end.
   Hint Unfold subset.
+  Notation "s1 ⊂ s2" := (subset s1 s2) (at level 70, no associativity).
 
-  Theorem subset_nil : forall s, subset nil s.
+  Theorem subset_nil : forall s, nil ⊂ s.
   Proof.
     auto.
   Qed.
 
-  Theorem subset_nil_nil : forall s, subset s nil -> s = nil.
+  Theorem subset_nil_nil : forall s, s ⊂ nil -> s = nil.
   Proof.
     induction s.
     auto.
@@ -361,10 +376,10 @@ Section Sets.
     inversion H.
   Qed.
 
-  Definition set_eq s1 s2 := subset s1 s2 /\ subset s2 s1.
+  Definition set_eq s1 s2 := s1 ⊂ s2 /\ s2 ⊂ s1.
   Hint Unfold set_eq.
 
-  Lemma subset_consr s1 s2 n : subset s1 s2 -> subset s1 (cons n s2).
+  Lemma subset_consr s1 s2 n : s1 ⊂ s2 -> s1 ⊂ (cons n s2).
   Proof.
     generalize dependent s2.
     generalize dependent n.
@@ -382,7 +397,7 @@ Section Sets.
     apply IHs1; auto.
   Defined.
 
-  Definition subset_dec s1 s2 : { subset s1 s2 } + { ~ (subset s1 s2) }.
+  Definition subset_dec s1 s2 : { s1 ⊂ s2 } + { ~ (s1 ⊂ s2) }.
   Proof.
     generalize dependent s2.
     induction s1.
@@ -402,7 +417,7 @@ Section Sets.
     intros H; destruct H; contradiction.
   Defined.
 
-  Definition subset_nn s1 s2 : ~~(subset s1 s2) -> subset s1 s2.
+  Definition subset_nn s1 s2 : ~~(s1 ⊂ s2) -> s1 ⊂ s2.
   Proof.
     destruct (subset_dec s1 s2); tauto.
   Qed.
@@ -416,7 +431,7 @@ Section Sets.
     right; intros contra; destruct contra; apply n; auto.
   Qed.
 
-  Theorem subset_refl s : subset s s.
+  Theorem subset_refl s : s ⊂ s.
   Proof.
     induction s; unfold subset; auto.
     fold subset.
@@ -430,7 +445,7 @@ Section Sets.
     split; apply subset_refl.
   Qed.
 
-  Theorem subset_In : forall x s s', set_In x s -> subset s s' -> set_In x s'.
+  Theorem subset_In : forall x s s', set_In x s -> s ⊂ s' -> set_In x s'.
   Proof.
     intros x s.
     generalize dependent x.
@@ -443,7 +458,7 @@ Section Sets.
     destruct Hyinxs; subst; auto.
   Qed.
 
-  Theorem subset_In_def s s' : (forall x, set_In x s -> set_In x s') -> subset s s'.
+  Theorem subset_In_def s s' : (forall x, set_In x s -> set_In x s') -> s ⊂ s'.
   Proof.
     generalize dependent s'.
     induction s.
@@ -457,7 +472,7 @@ Section Sets.
     constructor 2; auto.
   Qed.
 
-  Theorem In_subset_def s s' : subset s s' -> (forall x, set_In x s -> set_In x s').
+  Theorem In_subset_def s s' : s ⊂ s' -> (forall x, set_In x s -> set_In x s').
   Proof.
     generalize dependent s'.
     induction s.
@@ -475,23 +490,23 @@ Section Sets.
   Qed.
 
   Hint Resolve subset_In_def In_subset_def.
-  Theorem subset_In_equiv s s' : subset s s' <-> (forall x, set_In x s -> set_In x s').
+  Theorem subset_In_equiv s s' : s ⊂ s' <-> (forall x, set_In x s -> set_In x s').
   Proof.
     split; eauto.
   Qed.
 
-  Lemma set_subset_weaken : forall s1 s2, set_eq s1 s2 -> subset s1 s2.
+  Lemma set_subset_weaken : forall s1 s2, set_eq s1 s2 -> s1 ⊂ s2.
   Proof.
     unfold set_eq.
     tauto.
   Qed.
 
-  Theorem not_subset_In_def s s' x : set_In x s -> ~(set_In x s') -> ~ subset s s'.
+  Theorem not_subset_In_def s s' x : set_In x s -> ~(set_In x s') -> ~ s ⊂ s'.
   Proof.
     intros; eauto.
   Qed.
 
-  Lemma subset_trans : forall s1 s2 s3, subset s1 s2 -> subset s2 s3 -> subset s1 s3.
+  Lemma subset_trans : forall s1 s2 s3, s1 ⊂ s2 -> s2 ⊂ s3 -> s1 ⊂ s3.
   Proof.
     intros s1.
     induction s1 as [| x s1].
@@ -525,9 +540,9 @@ Section Sets.
     intros s1 s2 H; inversion H; split; auto.
   Qed.
 
-  (* Theorem set_union_or : forall s1 s2, subset s1 (s1 ∪ s2). *)
+  (* Theorem set_union_or : forall s1 s2, s1 ⊂ (s1 ∪ s2). *)
 
-  Lemma set_add_subset : forall x s1 s2, set_In x s2 -> subset s1 s2 -> subset (set_add' x s1) s2.
+  Lemma set_add_subset : forall x s1 s2, set_In x s2 -> s1 ⊂ s2 -> (set_add' x s1) ⊂ s2.
   Proof.
 
     intros y s1.
@@ -545,7 +560,7 @@ Section Sets.
     destruct Hsub; auto.
   Qed.
 
-  Lemma subset_cons_swap : forall x y s1 s2, subset s1 s2 -> subset (x :: y :: s1) (y :: x :: s2).
+  Lemma subset_cons_swap : forall x y s1 s2, s1 ⊂ s2 -> (x :: y :: s1) ⊂ (y :: x :: s2).
   Proof.
     intros x y s1 s2.
     destruct (eq_nat_dec x y).
@@ -572,7 +587,7 @@ Section Sets.
     split; destruct H; apply subset_cons_swap; auto.
   Qed.
 
-  Lemma set_cons_cons_subset : forall x s1 s2, subset s1 s2 -> subset (x :: s1) (x :: s2).
+  Lemma set_cons_cons_subset : forall x s1 s2, s1 ⊂ s2 -> (x :: s1) ⊂ (x :: s2).
   Proof.
     intros x s1 s2 Hsub.
     unfold subset. fold subset.
@@ -632,7 +647,7 @@ Section Sets.
     apply subset_refl.
   Qed.
 
-  Lemma set_add_cons_subset : forall x s1 s2, subset s1 s2 -> subset (x :: s1) (set_add' x s2).
+  Lemma set_add_cons_subset : forall x s1 s2, s1 ⊂ s2 -> (x :: s1) ⊂ (set_add' x s2).
   Proof.
     intros x s1 s2 Hsub.
     apply subset_trans with (s2 := (x :: s2)).
@@ -692,7 +707,7 @@ Section Sets.
     auto.
   Qed.
 
-  Lemma subset_union_cons : forall x s1 s2, subset ((x::s1) ∪ s2) (x :: (s1 ∪ s2)).
+  Lemma subset_union_cons : forall x s1 s2, ((x::s1) ∪ s2) ⊂ (x :: (s1 ∪ s2)).
     induction s2.
     simpl; split.
     tauto.
@@ -710,7 +725,7 @@ Section Sets.
     apply set_add_cons_eq.
   Qed.
 
-  Theorem subset_union_comm : forall s1 s2, subset (s1 ∪ s2) (s2 ∪ s1).
+  Theorem subset_union_comm : forall s1 s2, (s1 ∪ s2) ⊂ (s2 ∪ s1).
   Proof.
     induction s1.
     intros.
@@ -734,8 +749,8 @@ Section Sets.
 
   Lemma subset_union_transr :
     forall s sl sr,
-      subset s sr ->
-      subset s (sl ∪ sr).
+      s ⊂ sr ->
+      s ⊂ (sl ∪ sr).
   Proof.
     intros.
     apply subset_In_def.
@@ -748,8 +763,8 @@ Section Sets.
 
   Lemma subset_union_transl :
     forall s sl sr,
-      subset s sl ->
-      subset s (sl ∪ sr).
+      s ⊂ sl ->
+      s ⊂ (sl ∪ sr).
   Proof.
     intros.
     eapply subset_trans; [| apply subset_union_comm ].
@@ -759,7 +774,7 @@ Section Sets.
 
   Lemma set_union_subset_cong :
     forall sl sr sl' sr',
-      subset sl sl' -> subset sr sr' -> subset (sl ∪ sr) (sl' ∪ sr').
+      sl ⊂ sl' -> sr ⊂ sr' -> (sl ∪ sr) ⊂ (sl' ∪ sr').
   Proof.
     induction sr.
     intros.
@@ -794,7 +809,7 @@ Section Sets.
   Qed.
 
 
-  Lemma set_subset_add : forall x s1 s2, subset s1 s2 -> subset s1 (set_add' x s2).
+  Lemma set_subset_add : forall x s1 s2, s1 ⊂ s2 -> s1 ⊂ (set_add' x s2).
   Proof.
     intros x s1 s2 Hsub.
     eapply subset_trans; [| apply set_add_cons_subset; apply subset_refl ].
@@ -840,7 +855,7 @@ Section Sets.
 
 
   Theorem subset_union_both s sl sr
-  : subset sl s -> subset sr s -> subset (sl ∪ sr) s.
+  : sl ⊂ s -> sr ⊂ s -> (sl ∪ sr) ⊂ s.
   Proof.
     intros Hls Hrs.
     apply subset_In_def.
@@ -851,7 +866,7 @@ Section Sets.
     apply In_subset_def with sr; auto.
   Qed.
 
-  Theorem subset_union_eq : forall s1 s2, subset s1 s2 -> set_eq (s1 ∪ s2) s2.
+  Theorem subset_union_eq : forall s1 s2, s1 ⊂ s2 -> set_eq (s1 ∪ s2) s2.
   Proof.
     split; [| apply subset_union_transr; apply subset_refl ].
     generalize dependent s2.
@@ -898,7 +913,7 @@ Section Sets.
     tauto.
   Qed.
 
-  Lemma subset_app : forall s1 s2 s3, subset s1 s2 -> subset s1 (s2 ++ s3).
+  Lemma subset_app : forall s1 s2 s3, s1 ⊂ s2 -> s1 ⊂ (s2 ++ s3).
   Proof.
     induction s1; auto.
     induction s2.
@@ -926,7 +941,7 @@ Section Sets.
 
     apply IHs1; auto.
   Qed.
-  Lemma subset_rev : forall s, subset s (rev s).
+  Lemma subset_rev : forall s, s ⊂ (rev s).
   Proof.
     induction s; auto.
     constructor.
@@ -986,7 +1001,7 @@ Section Sets.
     nliamega.
   Qed.
 
-  Lemma z_to_n_nosubS m : ~ subset (z_to_n (S m)) (z_to_n m).
+  Lemma z_to_n_nosubS m : ~ (z_to_n (S m)) ⊂ (z_to_n m).
   Proof.
     intros H.
     assert (set_In m (z_to_n m)).
@@ -996,7 +1011,7 @@ Section Sets.
     nliamega.
   Qed.
 
-  Lemma z_to_n_nosub' m n : ~ subset (z_to_n (S (m + n))) (z_to_n m).
+  Lemma z_to_n_nosub' m n : ~ (z_to_n (S (m + n))) ⊂ (z_to_n m).
   Proof.
     induction n.
     replace (m + 0) with m by nliamega.
@@ -1018,7 +1033,7 @@ Section Sets.
     auto.
   Qed.
 
-  Lemma z_to_n_nosub m n : m < n -> ~ subset (z_to_n n) (z_to_n m).
+  Lemma z_to_n_nosub m n : m < n -> ~ (z_to_n n) ⊂ (z_to_n m).
   Proof.
     intros H1 H2.
     destruct n; [nliamega|].
@@ -1030,8 +1045,8 @@ Section Sets.
     rewrite !z_to_n_correct; auto.
   Qed.
 
-
 End Sets.
+Notation "s1 ⊂ s2" := (subset s1 s2) (at level 70, no associativity).
 Hint Resolve set_eq_refl.
 Hint Resolve subset_refl.
 
@@ -1059,7 +1074,7 @@ Section Traces.
       | (Tracing l1 l2 l3 l4, Tracing r1 r2 r3 r4) =>
         Tracing (l1 ∪ r1) (l2 ∪ r2) (l3 ∪ r3) (l4 ∪ r4)
     end.
-  Notation "x +++ y" := (trace_plus x y) (at level 50).
+  Notation "x ⊕ y" := (trace_plus x y) (at level 50).
 
   Definition trace_one n t : Trace :=
     match t with
@@ -1082,10 +1097,7 @@ Section Traces.
   Definition sub_trace (t1 t2 : Trace) : Prop :=
     match (t1, t2) with
       | (Tracing l0 l1 l2 l3, Tracing r0 r1 r2 r3) =>
-        subset l0 r0
-        /\ subset l1 r1
-        /\ subset l2 r2
-        /\ subset l3 r3
+        l0 ⊂ r0 /\ l1 ⊂ r1 /\ l2 ⊂ r2 /\ l3 ⊂ r3
     end.
 
   Theorem sub_trace_refl t : sub_trace t t.
@@ -1108,7 +1120,7 @@ Section Traces.
     unfold trace_eq, trace_proj; destruct t1; destruct t2; destruct tg; intuition.
   Qed.
 
-  Theorem sub_trace_proj t1 t2 tg : sub_trace t1 t2 -> subset (trace_proj tg t1) (trace_proj tg t2).
+  Theorem sub_trace_proj t1 t2 tg : sub_trace t1 t2 -> (trace_proj tg t1) ⊂ (trace_proj tg t2).
   Proof.
     unfold sub_trace; destruct t1; destruct t2; destruct tg; intuition.
   Qed.
@@ -1131,7 +1143,7 @@ Section Traces.
   Theorem trace_eq_weakenr t1 t2 : t1 ≡ t2 -> sub_trace t2 t1.
   Proof. rewrite trace_eq_eq'_equiv; apply trace_eq'_weakenr. Qed.
 
-  Theorem trace_plus_cong t1 t2 t3 t4 : t1 ≡ t3 -> t2 ≡ t4 -> (t1 +++ t2) ≡ (t3 +++ t4).
+  Theorem trace_plus_cong t1 t2 t3 t4 : t1 ≡ t3 -> t2 ≡ t4 -> (t1 ⊕ t2) ≡ (t3 ⊕ t4).
     unfold trace_eq.
     destruct t1; destruct t2; destruct t3; destruct t4.
     unfold trace_plus.
@@ -1163,15 +1175,15 @@ Section Traces.
     split4; eapply set_eq_trans; eauto.
   Qed.
 
-  Theorem trace_plus_comm t1 t2 : (t1 +++ t2) ≡ (t2 +++ t1).
+  Theorem trace_plus_comm t1 t2 : (t1 ⊕ t2) ≡ (t2 ⊕ t1).
   Proof.
     destruct t1, t2.
     unfold trace_plus.
     split4; apply set_eq_union_comm.
   Qed.
 
-  Theorem trace_plus_assoc t1 t2 t3 : (t1 +++ (t2 +++ t3)) ≡
-                                               ((t1 +++ t2) +++ t3).
+  Theorem trace_plus_assoc t1 t2 t3 : (t1 ⊕ (t2 ⊕ t3)) ≡
+                                               ((t1 ⊕ t2) ⊕ t3).
   Proof.
     destruct t1, t2, t3.
     unfold trace_plus.
@@ -1179,14 +1191,14 @@ Section Traces.
   Qed.
 
   Theorem sub_trace_plus_transl t tl tr
-  : sub_trace t tl -> sub_trace t (tl +++ tr).
+  : sub_trace t tl -> sub_trace t (tl ⊕ tr).
   Proof.
     intros H; destruct t; destruct tl; destruct tr;
     destruct4 H; split4; apply subset_union_transl; auto.
   Qed.
 
   Theorem sub_trace_plus_transr t tl tr
-  : sub_trace t tr -> sub_trace t (tl +++ tr).
+  : sub_trace t tr -> sub_trace t (tl ⊕ tr).
   Proof.
     intros H.
     eapply sub_trace_trans.
@@ -1196,20 +1208,20 @@ Section Traces.
     apply sub_trace_plus_transl; auto.
   Qed.
 
-  Theorem sub_trace_plus_eq : forall t1 t2, sub_trace t1 t2 -> (t1 +++ t2) ≡ t2.
+  Theorem sub_trace_plus_eq : forall t1 t2, sub_trace t1 t2 -> (t1 ⊕ t2) ≡ t2.
   Proof.
     intros t1 t2 H; destruct t1; destruct t2;
       destruct4 H; split4; apply subset_union_eq; auto.
   Qed.
 
   Theorem trace_plus_unitl t :
-    (trace_zero +++ t) ≡ t.
+    (trace_zero ⊕ t) ≡ t.
   Proof.
     destruct t; split4; apply set_union_unitl.
   Qed.
 
   Theorem trace_plus_unitl_gen t1 t2 :
-    t1 ≡ t2 -> (trace_zero +++ t1) ≡ t2.
+    t1 ≡ t2 -> (trace_zero ⊕ t1) ≡ t2.
   Proof.
     intros H.
     eapply trace_eq_trans; [ apply trace_plus_unitl | auto].
@@ -1217,7 +1229,7 @@ Section Traces.
 
 
   Theorem trace_plus_unitr t :
-    (t +++ trace_zero) ≡ t.
+    (t ⊕ trace_zero) ≡ t.
   Proof.
     eapply trace_eq_trans;
     [apply trace_plus_comm| apply trace_plus_unitl].
@@ -1225,7 +1237,7 @@ Section Traces.
 
 
   Theorem trace_plus_unitr_gen t1 t2 :
-    t1 ≡ t2 -> (t1 +++ trace_zero) ≡ t2.
+    t1 ≡ t2 -> (t1 ⊕ trace_zero) ≡ t2.
   Proof.
     intros H.
     eapply trace_eq_trans; [ apply trace_plus_unitr | auto].
@@ -1234,7 +1246,7 @@ Section Traces.
   Theorem sub_trace_plus_cong tl1 tr1 tl2 tr2 : 
   sub_trace tl1 tl2
   -> sub_trace tr1 tr2
-  -> sub_trace (tl1 +++ tr1) (tl2 +++ tr2).
+  -> sub_trace (tl1 ⊕ tr1) (tl2 ⊕ tr2).
   Proof.
     unfold sub_trace, trace_plus.
     destruct tl1; destruct tl2; destruct tr1; destruct tr2.
@@ -1272,7 +1284,7 @@ Section Traces.
   Qed.
 
 End Traces.
-Notation "x +++ y" := (trace_plus x y) (at level 50).
+Notation "x ⊕ y" := (trace_plus x y) (at level 50).
 Notation "t1 ≡ t2" := (trace_eq t1 t2) (at level 70, no associativity).
 Hint Resolve trace_eq_refl.
 Hint Resolve sub_trace_refl.
@@ -1287,7 +1299,7 @@ Section Enumerates.
         Pairing n ln rn ->
         Enumerates l ln lx lt ->
         Enumerates r rn rx rt ->
-        Enumerates (E_Pair l r) n (V_Pair lx rx) (lt +++ rt)
+        Enumerates (E_Pair l r) n (V_Pair lx rx) (lt ⊕ rt)
   | ES_Map :
       forall bi inner inner_x n x t,
         Bijects bi x inner_x ->
@@ -1298,7 +1310,7 @@ Section Enumerates.
         Pairing n ln rn ->
         Enumerates l ln lx lt ->
         Enumerates (f lx) rn rx rt ->
-        Enumerates (E_Dep l f) n (V_Pair lx rx) (lt +++ rt)
+        Enumerates (E_Dep l f) n (V_Pair lx rx) (lt ⊕ rt)
   | ES_Sum_Left:
       forall l r n ln lx t,
         n = 2 * ln ->
@@ -1493,7 +1505,7 @@ Section Enumerates.
       destruct (IHe2 rx) as [[[rn rt] ER] | RF].
       left.
       destruct (Pairing_to_dec ln rn) as [n P].
-      exists (n, lt +++ rt).
+      exists (n, lt ⊕ rt).
       eauto.
 
       right. intros _n _t E; inversion E; subst.
@@ -1507,7 +1519,7 @@ Section Enumerates.
       destruct (X x1 x2) as [[[rn rt] ER] | RF].
       left.
       destruct (Pairing_to_dec ln rn) as [n P].
-      exists (n, lt +++ rt).
+      exists (n, lt ⊕ rt).
       eauto.
 
       right. intros _n _t E; inversion E; subst.
@@ -1582,7 +1594,7 @@ Section Enumerates.
       destruct PF as [ln rn].
       destruct (IHe1 ln) as [[lx lt] EL].
       destruct (IHe2 rn) as [[rx rt] ER].
-      exists (V_Pair lx rx, lt +++ rt).
+      exists (V_Pair lx rx, lt ⊕ rt).
       eauto.
 
     (* E_Map *)
@@ -1596,7 +1608,7 @@ Section Enumerates.
       destruct PF as [ln rn].
       destruct (IHe ln) as [[lx lt] EL].
       destruct (X lx rn) as [[rx rt] ER].
-      exists (V_Pair lx rx, lt +++ rt). eauto.
+      exists (V_Pair lx rx, lt ⊕ rt). eauto.
 
     (* E_Sum *)
     - destruct (even_odd_dec n) as [Hev | Hodd].
@@ -1632,7 +1644,7 @@ Section EnumTrace.
   Fixpoint Trace_lt (e : Enum) n : Trace :=
     match n with
       | 0 => trace_zero
-      | S n' => (Trace_on e n') +++ (Trace_lt e n')
+      | S n' => (Trace_on e n') ⊕ (Trace_lt e n')
     end.
 
   Fixpoint Trace_from_to e lo hi : Trace :=
@@ -1640,7 +1652,7 @@ Section EnumTrace.
     then trace_zero
     else match hi with
            | 0 => trace_zero
-           | S hi' => (Trace_on e hi') +++ (Trace_from_to e lo hi')
+           | S hi' => (Trace_on e hi') ⊕ (Trace_from_to e lo hi')
          end.
 
   Theorem trace_lt_from_to_0_same e n : (Trace_lt e n) ≡ (Trace_from_to e 0 n).
@@ -1675,7 +1687,7 @@ Section EnumTrace.
 
   Theorem trace_from_to_split1r e m n
   : m <= n ->
-    (Trace_from_to e m (S n)) ≡ ((Trace_from_to e m n) +++ (Trace_on e n)).
+    (Trace_from_to e m (S n)) ≡ ((Trace_from_to e m n) ⊕ (Trace_on e n)).
   Proof.
     intros H.
     unfold Trace_from_to at 1.
@@ -1690,7 +1702,7 @@ Section EnumTrace.
   Qed.
 
   Theorem trace_from_to_split1l' e m n
-  : (Trace_from_to e m (S (m + n))) ≡ ((Trace_on e m) +++ (Trace_from_to e (S m) (S (m + n)))).
+  : (Trace_from_to e m (S (m + n))) ≡ ((Trace_on e m) ⊕ (Trace_from_to e (S m) (S (m + n)))).
   Proof.
     generalize dependent m.
     induction n as [| n].
@@ -1738,7 +1750,7 @@ Section EnumTrace.
 
   Theorem trace_from_to_split1l e m n
   : m < n ->
-    Trace_from_to e m n ≡ (Trace_on e m) +++ (Trace_from_to e (S m) n).
+    Trace_from_to e m n ≡ (Trace_on e m) ⊕ (Trace_from_to e (S m) n).
   Proof.
     intros H.
     remember (pred (n - m)) as t.
@@ -1750,7 +1762,7 @@ Section EnumTrace.
 
   Theorem trace_from_to_split e m n p :
     (m <= n < p)
-    -> Trace_from_to e m p ≡ (Trace_from_to e m n) +++ (Trace_from_to e n p).
+    -> Trace_from_to e m p ≡ (Trace_from_to e m n) ⊕ (Trace_from_to e n p).
   Proof.
     generalize dependent p.
     generalize dependent m.
@@ -1771,10 +1783,10 @@ Section EnumTrace.
     apply trace_plus_unitl_gen.
     apply trace_eq_refl.
 
-    apply trace_eq_trans with ((Trace_from_to e m n) +++ (Trace_from_to e n p));
+    apply trace_eq_trans with ((Trace_from_to e m n) ⊕ (Trace_from_to e n p));
       [apply IHn; nliamega| ].
     apply trace_eq_trans with ((Trace_from_to e m n)
-                                 +++ ((Trace_on e n) +++ (Trace_from_to e (S n) p))).
+                                 ⊕ ((Trace_on e n) ⊕ (Trace_from_to e (S n) p))).
     apply trace_plus_cong; [apply trace_eq_refl| ].
     apply trace_from_to_split1l; nliamega.
 
@@ -1788,7 +1800,7 @@ Section EnumTrace.
   Theorem trace_from_to_0_split :
     forall m n e,
       m < n ->
-      Trace_lt e n ≡ (Trace_lt e m) +++ (Trace_from_to e m n).
+      Trace_lt e n ≡ (Trace_lt e m) ⊕ (Trace_from_to e m n).
   Proof.
     intros m n e Hmn.
     eapply trace_eq_trans.
@@ -1817,7 +1829,7 @@ Section EnumTrace.
   Qed.
 
   Theorem trace_proj_plus_distrl tg t1 t2
-  : trace_proj tg (t1 +++ t2) = ((trace_proj tg t1) ∪ (trace_proj tg t2)).
+  : trace_proj tg (t1 ⊕ t2) = ((trace_proj tg t1) ∪ (trace_proj tg t2)).
   Proof.
     destruct t1; destruct t2; destruct tg; auto.
   Qed.
@@ -1984,7 +1996,7 @@ Section EnumTrace.
                         |
                         fold Trace_from_to in H;
                           rewrite trace_from_to_self in H;
-                          remember ((Trace_on e m) +++ trace_zero) as t;
+                          remember ((Trace_on e m) ⊕ trace_zero) as t;
                           destruct t;
                           simpl in *;
                           remember (Trace_on e m) as t';
@@ -2015,7 +2027,7 @@ Section EnumTrace.
       destruct (le_lt_dec (S m) m); [apply le_Sn_n in l; contradiction|];
       fold Trace_from_to; rewrite trace_from_to_self; assert (k = m) by nliamega; subst;
 
-      remember ((Trace_on e m) +++ trace_zero) as t;
+      remember ((Trace_on e m) ⊕ trace_zero) as t;
       destruct t; simpl in *;
       remember (Trace_on e m) as t';
       destruct t';
@@ -2070,7 +2082,7 @@ Section EnumTrace.
   Qed.
 
   Theorem sub_trace_plus_introl t1 t2 t3
-  : sub_trace t1 t2 -> sub_trace t1 (t2 +++ t3).
+  : sub_trace t1 t2 -> sub_trace t1 (t2 ⊕ t3).
   Proof.
     unfold sub_trace, trace_plus; destruct t1, t2, t3.
     intros H; destruct H as [H1 [H2 [H3 H4]]].
@@ -2079,7 +2091,7 @@ Section EnumTrace.
   Qed.
 
   Theorem sub_trace_plus_intror t1 t2 t3
-  : sub_trace t1 t3 -> sub_trace t1 (t2 +++ t3).
+  : sub_trace t1 t3 -> sub_trace t1 (t2 ⊕ t3).
   Proof.
     unfold sub_trace, trace_plus; destruct t1, t2, t3.
     intros H; destruct H as [H1 [H2 [H3 H4]]].
@@ -2186,7 +2198,7 @@ Section Fairness.
   Section SumFair.
     Lemma Sum_precise
     : forall n e1 e2,
-        Trace_lt (E_Sum e1 e2) (double n) ≡ (Trace_lt e1 n) +++ (Trace_lt e2 n).
+        Trace_lt (E_Sum e1 e2) (double n) ≡ (Trace_lt e1 n) ⊕ (Trace_lt e2 n).
     Proof.
       intros n e1 e2.
       induction n.
@@ -2350,7 +2362,7 @@ Section Fairness.
     Lemma SumSum_precise
     : forall n e1 e2 e3,
         Trace_lt (E_Sum e1 (E_Sum e2 e3)) (double (double n))
-        ≡ (Trace_lt e1 (double n)) +++ ((Trace_lt e2 n) +++ (Trace_lt e3 n)).
+        ≡ (Trace_lt e1 (double n)) ⊕ ((Trace_lt e2 n) ⊕ (Trace_lt e3 n)).
     Proof.
       intros.
       eapply trace_eq_trans; [apply Sum_precise|].
@@ -2402,15 +2414,15 @@ Section Fairness.
       assert (exists m p, 2 * m <= n < 4 * p /\ p < m) as [m [p [[Hmn Hnp] Hpn]]] by (apply div2div4; nliamega).
       left.
       
-      assert (~ subset s0 s1); [| intros [? ?]; contradiction ].
+      assert (~ s0 ⊂ s1); [| intros [? ?]; contradiction ].
 
-      assert (subset (z_to_n m) s0).
+      assert ((z_to_n m) ⊂ s0).
       rewrite <-double_twice in *.
       replace s0 with (trace_proj zero (Trace_lt NS3T n)) by (rewrite <-Heqt; trivial).
       eapply subset_trans; [| apply sub_trace_proj; apply Trace_lt_sub; apply Hmn ].
       apply set_subset_weaken; apply set_eq_symm; apply NS3Tl_precise.
       
-      assert (subset s1 (z_to_n p)).
+      assert (s1 ⊂ (z_to_n p)).
       replace (4 * p) with (double (double p)) in * by (simpl; unfold double; nliamega).
       replace s1 with (trace_proj one (Trace_lt NS3T n)) by (rewrite <-Heqt; trivial).
       eapply subset_trans.
@@ -2429,7 +2441,7 @@ Section Fairness.
     Definition E_PairNN := (E_Pair (E_Trace zero E_Nat) (E_Trace one E_Nat)).
     Lemma Pair_layer e1 e2 n
     : Trace_from_to (E_Pair e1 e2) (n * n) (S n * S n)
-      ≡ (Trace_lt e1 (S n)) +++ (Trace_lt e2 (S n)).
+      ≡ (Trace_lt e1 (S n)) ⊕ (Trace_lt e2 (S n)).
     Proof.
       apply trace_eq_eq'_equiv; split.
       (* trace (e1 x e2) n^2 (n+1)^2 < (trace ) *)
@@ -2440,8 +2452,8 @@ Section Fairness.
         destruct (Enumerates_from_dec (E_Pair e1 e2) k) as [[v t] Henum].
         inversion Henum; subst.
         simpl in Hin.
-        destruct (sub_trace_In_equiv (lt +++ rt)
-                                     ((Trace_lt e1 (S n)) +++ (Trace_lt e2 (S n)))).
+        destruct (sub_trace_In_equiv (lt ⊕ rt)
+                                     ((Trace_lt e1 (S n)) ⊕ (Trace_lt e2 (S n)))).
         apply H; [| assumption].
         clear H H0.
         apply sub_trace_plus_cong;
@@ -2489,7 +2501,7 @@ Section Fairness.
       unfold E_PairNN; apply Pair_layer.
       apply trace_eq_symm.
       apply trace_eq_trans with ((Tracing (z_to_n (S n)) ∅ ∅ ∅)
-                                   +++ (Tracing ∅ (z_to_n (S n)) ∅ ∅)).
+                                   ⊕ (Tracing ∅ (z_to_n (S n)) ∅ ∅)).
       remember (S n) as k; unfold trace_plus; split4; auto; apply set_eq_symm; apply set_union_unitl.
       apply trace_plus_cong; rewrite trace_proj_reconstruct.
       split4; [ apply trace_lt_Nat | | | ]; rewrite trace_lt_Nat_off by discriminate; auto.
@@ -2498,7 +2510,7 @@ Section Fairness.
 
     Lemma Pair_precise
     : forall n e1 e2,
-        (Trace_lt (E_Pair e1 e2) (n * n)) ≡ ((Trace_lt e1 n) +++ (Trace_lt e2 n)).
+        (Trace_lt (E_Pair e1 e2) (n * n)) ≡ ((Trace_lt e1 n) ⊕ (Trace_lt e2 n)).
       intros n.
       induction n as [| n IHn]; [  intros; compute; tauto| ].
       intros e1 e2.
@@ -2513,7 +2525,7 @@ Section Fairness.
     Lemma PairPair_precise
     : forall n e1 e2 e3,
         Trace_lt (E_Pair e1 (E_Pair e2 e3)) ((n * n) * (n * n))
-        ≡ (Trace_lt e1 (n * n)) +++ ((Trace_lt e2 n) +++ (Trace_lt e3 n)).
+        ≡ (Trace_lt e1 (n * n)) ⊕ ((Trace_lt e2 n) ⊕ (Trace_lt e3 n)).
     Proof.
       intros n e1 e2 e3.
       eapply trace_eq_trans; [apply Pair_precise|].
@@ -2527,10 +2539,10 @@ Section Fairness.
       induction n.
       compute; tauto.
       apply trace_eq_trans
-      with (t2 := ((Trace_lt E_PairNN (n * n)) +++ (Trace_from_to E_PairNN (n * n) (S n * S n)))).
+      with (t2 := ((Trace_lt E_PairNN (n * n)) ⊕ (Trace_from_to E_PairNN (n * n) (S n * S n)))).
       apply trace_from_to_0_split; nliamega.
       apply trace_eq_trans with (t2 := ((Tracing (z_to_n n) (z_to_n n) ∅ ∅)
-                                        +++ (Tracing (z_to_n (S n)) (z_to_n (S n)) ∅ ∅))).
+                                        ⊕ (Tracing (z_to_n (S n)) (z_to_n (S n)) ∅ ∅))).
       apply trace_plus_cong; auto.
       apply PairNN_layer.
       apply trace_eq_trans with (t2 := (Tracing (z_to_n (S n)) (z_to_n (S n))) ∅ ∅).
@@ -2585,9 +2597,9 @@ Section Fairness.
       destruct (sqrt_4th_root_spread n) as [m [p [[Hmn Hnp] Hppmm]]]; auto.
 
       left.
-      assert (~ subset t0 t1); [ | intros []; contradiction].
+      assert (~ t0 ⊂ t1); [ | intros []; contradiction].
 
-      assert (subset (z_to_n m) t0).
+      assert ((z_to_n m) ⊂ t0).
       - remember (Trace_lt NP3T (m * m)) as t; destruct t as [mm0 mm1 mm2 mm3].
         assert (sub_trace (Trace_lt NP3T (m * m)) (Trace_lt NP3T n))
           by (apply Trace_lt_sub; auto).
@@ -2601,7 +2613,7 @@ Section Fairness.
         remember (Pair_precise m (E_Trace zero E_Nat) (E_Pair (E_Trace one E_Nat) (E_Trace two E_Nat))).
         clear Heqt.
         rewrite <-Heqt0 in t.
-        remember (((Trace_lt (E_Trace zero E_Nat) m) +++ (Trace_lt (E_Pair (E_Trace one E_Nat) (E_Trace two E_Nat)) m))).
+        remember (((Trace_lt (E_Trace zero E_Nat) m) ⊕ (Trace_lt (E_Pair (E_Trace one E_Nat) (E_Trace two E_Nat)) m))).
         destruct t0.
         replace mm0 with (trace_proj zero (Tracing mm0 mm1 mm2 mm3)) by auto.
         eapply subset_trans; [| apply trace_eq_proj;  eassumption].
@@ -2610,7 +2622,7 @@ Section Fairness.
         apply subset_union_transl.
         apply trace_lt_Nat.
 
-      - assert (subset t1 (z_to_n p)).
+      - assert (t1 ⊂ (z_to_n p)).
         remember (Trace_lt NP3T ((p * p) * (p * p))) as p4t.
         assert (sub_trace (Trace_lt NP3T n) p4t) by (subst; apply Trace_lt_sub; auto; nliamega).
         destruct p4t as [pt0 pt1 pt2 pt3].
